\documentclass{report}

\input{preamble}
\input{macros}
\input{letterfonts}

\title{\Huge{Math 115 QR \\
PSet 2}}
\author{\huge{Alex Hernandez Juarez}}
\date{July 17 2024}

\begin{document}

\maketitle
\newpage% or \cleardoublepage
% \pdfbookmark[<level>]{<title>}{<dest>}
\pdfbookmark[section]{\contentsname}{toc}
\tableofcontents
\pagebreak

\chapter{}
\section{Problem 3: Stewart 11.11.6}
\qs{}{(a) approximate $f$ by a Taylor polynomial with degree $n$ and number $a$. \\
(b) Use Taylor's inequality to estimate the accuracy of the approximation $f(x) = T_{n}(x)$ when x lies in the given interval}
\sol{
    \\
    (a) 
    \begin{center}
        \[ f(x) = \sin(x) \] 
        \[ a = \frac{\pi}{6}\]
        \[ n = 4 \]
        \[ 0 \leq x \leq \frac{\pi}{3}\]
        \[ f'(x) = \cos(x) \]
        \[ f''(x) = -\sin(x) \]    
        \[ f^{(3)}(x) = -\cos(x) \]
        \[ f^{(4)}(x) = \sin(x) \]
        \[ P_{4}(x) = \sin\left(\frac{\pi}{6}\right) + \cos\left(\frac{\pi}{6}\right) \left(x- \frac{\pi}{6}\right) + \frac{-\sin\left(\frac{\pi}{6}\right)}{2} \left(x-\frac{\pi}{6}\right)^{2} + \frac{-\cos\left(\frac{\pi}{6}\right)}{6} \left(x-\frac{\pi}{6}\right)^{3} + \frac{\sin\left(\frac{\pi}{6}\right)}{24} \left(x-\frac{\pi}{6}\right)^{4}\]   
        \[ T_{4}(x) = \frac{1}{2} + \frac{\sqrt{3}}{2} \left(x-\frac{\pi}{6}\right) - \frac{1}{4} \left(x-\frac{\pi}{6}\right)^{2} - \frac{\sqrt{3}}{12} \left(x-\frac{\pi}{6}\right)^{3} + \frac{1}{48} \left(x-\frac{\pi}{6}\right)^{4}\]  
    \end{center}
    (b) 
    \begin{center}
        \[ \left|f(x) = P_{n}(x) \right| \leq \frac{M(x-a)^{n+1}}{(n+1)!}\] 
        \[ \left|f(x) = P_{n}(x) \right| \leq \frac{1(0-\frac{\pi}{6})^{5}}{(5)!} \approx 0.000327953194429\] 
        \[ \left|f(x) = P_{n}(x) \right| \leq \frac{1(\frac{\pi}{3}-\frac{\pi}{6})^{5}}{(5)!} \approx 0.000327953194429\] 
    \end{center}
}

\section{Problem 4: Stewart 11.20}
\qs{}{(a) approximate $f$ by a Taylor polynomial with degree $n$ and number $a$. \\
(b) Use Taylor's inequality to estimate the accuracy of the approximation $f(x) = T_{n}(x)$ when x lies in the given interval}

\sol{
    \\
    (a) 
    \begin{center}
        \[ f(x) = x \ln(x) \] 
        \[ a = 1 \]
        \[ n = 3 \]
        \[ 0.5 \leq x \leq 1.5 \]   
        \[ f'(x) = 1 \cdot \ln(x) + x \frac{1}{x} = \ln(x) + 1\] 
        \[ f''(x) = \frac{1}{x} \cdot 1 + 0 \ln(x) = \frac{1}{x} = x^{-1}\]
        \[ f^{(3)} (x) = -x^{-2}\] 
        \[ P_{3}(x) = \ln(1) + (\ln(1) + 1) + (x-1) + \frac{(1)^{-1}}{2}(x-1)^{2} + \frac{-(1)^{-2}}{6}(x-1)^{3}\] 
        \[ T_{3}(x) = 0 + (x-1) + \frac{1}{2}(x-1)^2 + -\frac{1}{6}(x-1)^{3} \] 
    \end{center}
    (b)
    \[ f^{(4)} = 2(x)^{-3}\] 
    \[ \left|f(x) = P_{n}(x) \right| \leq \frac{M(x-a)^{n+1}}{(n+1)!}\] 
    \[ M = 2(0.5)^{-3} = 16\] 
    \[ |f(x) = P_{n}(x)| \leq \frac{16(0.5-1)^{4}}{4!} \approx 0.0416666666667 \]
    \[ |f(x) = P_{n}(x)| \leq \frac{16(1.5-1)^{4}}{4!} \approx 0.0416666666667\]
}

\section{Problem 5}
\qs{}{ (a) Use a second degree Taylor polynomial to approximate $\sqrt[5]{34}$. (It's up to you to pick a suitable
function to approximate and a suitable base for the approximation.) You should check that your
approximation is reasonable \\
(b) Use the Taylor Error Bound formula to find an upper bound on the error for the approximation
you made in part (a), and verify (using a calculator or computer) that your answer to part (a) is
indeed within this error bound \\
(c) Suppose you use the same Taylor polynomial as in part (a) to approximate $\sqrt[5]{30}$. Will the error
bound be the same? Why or why not? If not, find an upper bound on the error in using the
Taylor polynomial to approximate $\sqrt[5]{34}$.}

\sol{
    (a)
    \begin{center}
        \[ a = 32 \]
        \[ f(x) = (x)^{\frac{1}{5}}\]
        \[ f'(x) = \frac{1}{5}(x)^{\frac{-4}{5}}\]
        \[ f''(x) = \frac{-4}{25}x^{\frac{-9}{5}}\]   
        \[ P_{2}(x) = 32^{\frac{1}{5}} + \frac{1}{5}(32)^{-\frac{4}{5}} (x-32) - \frac{4}{50}(32)^{-\frac{9}{5}} (x-32)^{2} \] 
        \[ P_{2}(34) = 32^{\frac{1}{5}} + \frac{1}{5}(32)^{-\frac{4}{5}} (34-32) - \frac{4}{50}(32)^{-\frac{9}{5}} (34-32)^{2} \approx 2.024375 \] 
    \end{center}
    (b)
    \begin{center}
        \[[32,34]\] 
        \[ f^{(3)}(x) = \frac{36}{125}x^{-\frac{14}{5}}\] \
        \[ M = \frac{36}{125}\left(1\right)^{-\frac{14}{5}}\] 
        \[ \left|f(x) = P_{n}(x) \right| \leq \frac{M(x-a)^{n+1}}{(n+1)!}\] 
        \[ \left|f(x) = P_{n}(x) \right| \leq \frac{\frac{36}{125}\left(1\right)^{-\frac{14}{5}}(34-32)^{2+1}}{(2+1)!} \approx 0.0000234375\]
        \[ |\sqrt[5]{34} - 2.024375| = 0.0000224584998851\]
        \[ 0.0000224584998851 <  0.0000234375\]   
    \end{center}
    (c) \\
    It will be different because the M value is different 
}

\section{Problem: 6 Stewart 11.11.24} 

\qs{}{Use the information from Exercise 16 to estimate $\sin(38)$ correct to five decimal places}
\sol{
    \begin{center}
        \[ 38^{\circ} = \frac{\pi}{180} \cdot 38 = \frac{19 \pi}{90} = \frac{2\pi}{45} + \frac{\pi}{6}\] 
        \[ \frac{19 \pi }{90 } \text{ is in the range of } \left(0, \frac{\pi}{3}\right) \text{ so the approximation from question 3 should apply}\] 
        \[ 0.00001 \geq \frac{1\left(\frac{19\pi}{90} - \frac{\pi}{6}\right)^{n+1}}{(n + 1)!} \] 
        \[ 0.00001 \geq \frac{1\left(\frac{19\pi}{90} - \frac{\pi}{6}\right)^{4+1}}{(4 + 1)!} \approx 4.4223745988 \cdot 10^{7} \] 
        \[ T_{4}(x) = \frac{1}{2} + \frac{\sqrt{3}}{2} \left(\left(\frac{2\pi}{45} + \frac{\pi}{6}\right)-\frac{\pi}{6}\right) - \frac{1}{4} \left(\left(\frac{2\pi}{45} + \frac{\pi}{6}\right)-\frac{\pi}{6}\right)^{2} - \frac{\sqrt{3}}{12} \left(\left(\frac{2\pi}{45} + \frac{\pi}{6}\right)-\frac{\pi}{6}\right)^{3} + \frac{1}{48} \left(\left(\frac{2\pi}{45} + \frac{\pi}{6}\right)-\frac{\pi}{6}\right)^{4}\]  
        \[ T_{4}(x) = \frac{1}{2} + \frac{\sqrt{3}}{2} \left(\frac{2\pi}{45}\right) - \frac{1}{4} \left(\frac{2\pi}{45}\right)^{2} - \frac{\sqrt{3}}{12} \left(\frac{2\pi}{45}\right)^{3} + \frac{1}{48} \left(\frac{2\pi}{45}\right)^{4} \approx 0.61566\]  
    \end{center}
}

\section{Problem 7 }
\qs{}{Let $P_{n}(x)$ be the $n^{th}$ degree taylor polynomial for $f(x) = e^{x}$ based at $x = 0$. Use the error bound Taylor's inequality
to show that $\lim_{n \to \infty}|f(x) - P_{n}(x)| = 0$. }
\sol{
    \begin{center}
		\[ P_{n}(x) = e^{0} + e^{0}(x) + \frac{e^{0}}{2}(x)^{2} + \frac{e^{0}}{6}(x)^{3} + \frac{e^{0}}{24}(x)^{4} + \frac{e^{0}}{120}(x)^{5} + \ldots \frac{e^{0}}{n!}(x)^{n}\] 
		\[ P_{n}(x) = 1 + (x) + \frac{1}{2}(x)^{2} + \frac{1}{6}(x)^{3} + \frac{1}{24}(x)^{4} + \frac{1}{120}(x)^{5} + \ldots \frac{1}{n!}x^{n}\] 
		\[ P_{n}(x) = \sum^{n}_{k=0} \frac{1}{k!}(x)^{k}\]  
        \[ |f(x) - P_{n}(x)| \leq \frac{M(x-a)^{n+1}}{(n+1)!}\] 
		\[ |f(x) - P_{n}(x)| \leq \frac{e^{x}(x)^{n+1}}{(n+1)!}, \text{where } |e^{z}| \leq M \text{ for all } z \text{ between 0 and } x \] 
		\[ \lim_{n \to \infty} |f(x) - P_{n}(x) = ? \]
		\[ \lim_{n \to \infty } \frac{e^{x} \cdot x^{n+1}}{(n+1)!}\]  
		\[ e^{x} \lim_{n \to \infty } \frac{x^{n+1}}{(n+1)!} = 0 \] 
        \[ |f(x) - P_{n}(x)| \leq \frac{e^{x}(x)^{n+1}}{(n+1)!}, \text{where } |e^{0}| = M  \text{ between}  - \infty \text{ and } 0  \text{ for x} \] 
        \[ \lim_{n \to  \infty} |f(x) - P_{n}(x) = ? \]
		\[ \lim_{n \to  \infty } \frac{e^{0} \cdot x^{n+1}}{(n+1)!}\]  
		\[ \lim_{n \to   \infty } \frac{x^{n+1}}{(n+1)!} = 0 \] 

    \end{center}
}

\section{Problem 8}
\qs{}{Let $P_{n}(x)$ be the $n^{th}$ degree taylor polynomial for $f(x) = \frac{1}{1-x}$ based at $ x= 0$. It turns out that
$\lim_{n \to \infty} P_{n}(x) = f(x)$ for all $x$ in the interval $(-1,1)$ Can you show this using the method of the
previous problem? If not, what goes wrong? }
\sol{
    \begin{center}
        \[ f(x) = \frac{1}{1-x} = (1-x)^{-1}\]
        \[ f'(x) = (1-x)^{-2}\]
        \[ f''(x) = 2(1-x)^{-3} \]
        \[ f^{n}(x) = (n!)(1-x)^{-(n+1)}\]   
        \[ P_{n}(x) = (1-0)^{-1} - (1-0)^{-2} + \frac{2(1-0)^{-3}}{2} + \ldots + \frac{(-1)^{n}(n!)(1-0)^{-(n+1)}}{n!} (x)^{n}\] 
        \[ P_{n}(x) = (1)^{-1} - (1)^{-2}(x) + \frac{2(1)^{-3}}{2}(x)^{2} + \ldots + \frac{(-1)^{n}(n!)(1-0)^{-(n+1)}}{n!}(x)^{n}\] 
        \[ P_{n}(x) = \sum_{k=0}^{n} (1)^{-(n+1)}(x)^{k}\] 
        \[ |f(x) - P_{n}(x)| \leq \frac{M(x-a)^{n+1}}{(n+1)!}\] 
        \[ |f(x) - P_{n}(x)| \leq \frac{M(x-a)^{n+1}}{(n+1)!}, \text{where } |e^{z}| \leq M \text{ for all } z \text{ between 0 and } x \] 
    \end{center}
}
\end{document}

